{\bf 06.35}
Suppose $X_1, X_2$ are independent exponentially distributed random variables $X_i\sim$EXP($\theta$), and let $Y=X_1-X_2$.\\
(a) Find the MGF of $Y$.\\
We can think of $Y=X_1-X_2$ as $Y=X_1+(-1)X_2$. Then using Theorem 6.4.1,
\begin{eqnarray*}
 & = & (M_{X_1} (t))(M_{-X_2} (t))\\
 & = & (M_{X_1}(t))(M_{X_2}(-t))\\
 & = & \left(\frac{1}{1-\theta t}\right)\left(\frac{1}{1-\theta (-t)}\right)\\
 &=& \left(\frac{1}{1-\theta t}\right)\left(\frac{1}{1+\theta t}\right)\\
 & = & \frac{1}{1-\theta t +\theta t-\theta^2 t^2}\\
 & = & \frac{1}{1-\theta^2 t^2}
\end{eqnarray*}
(b) What is the distribution of $Y$?\\
Since $\frac{1}{1-\theta^2 t^2}$ is the MGF of a double exponential,  $Y\sim$ DE($\theta$,$0$).
\\
